lean investigation

lean_/mergeSort.lean
@@ -1,6 +1,6 @@
 -- TODO remove the `partial`s and convince Lean that mergeSort terminates
 
-partial def merge [Ord A] (xs : List A) (ys : List A) : List A :=
+def merge [Ord A] (xs : List A) (ys : List A) : List A :=
   match xs, ys with
   | [], _ => ys
   | _, [] => xs
@@ -8,22 +8,61 @@ partial def merge [Ord A] (xs : List A) (ys : List A) : List A :=
     match Ord.compare x' y' with
     | .lt | .eq => x' :: merge xs' (y' :: ys')
     | .gt => y' :: merge (x'::xs') ys'
+ termination_by merge xs ys => xs.length + ys.length
 
 def splitList (lst : List A) : (List A × List A) :=
   match lst with
-  | [] => ([], [])
+  | [] => ([], [])  --if list is empty returns a pair of empty lists
   | x :: xs =>
     let (a, b) := splitList xs
     (x :: b, a)
 
-partial def mergeSort [Ord A] (xs : List A) : List A :=
+theorem splitList_shorter_le (lst : List α) :
+    (splitList lst).fst.length ≤ lst.length ∧ (splitList lst).snd.length ≤ lst.length := by
+  induction lst with
+  | nil => simp [splitList]
+  | cons x xs ih =>
+    simp [splitList]
+    cases ih
+    constructor
+    case left => apply Nat.succ_le_succ; assumption
+    case right => apply Nat.le_succ_of_le; assumption
+
+theorem splitList_shorter (lst : List α) (_ : lst.length ≥ 2) :
+    (splitList lst).fst.length < lst.length ∧
+      (splitList lst).snd.length < lst.length := by
+  match lst with
+  | x :: y :: xs =>
+    simp_arith [splitList]
+    apply splitList_shorter_le
+
+theorem splitList_shorter_fst (lst : List α) (h : lst.length ≥ 2) :
+    (splitList lst).fst.length < lst.length :=
+  splitList_shorter lst h |>.left
+
+theorem splitList_shorter_snd (lst : List α) (h : lst.length ≥ 2) :
+    (splitList lst).snd.length < lst.length :=
+  splitList_shorter lst h |>.right
+
+def mergeSort [Ord A] (xs : List A) : List A :=
   if h : xs.length < 2 then
     match xs with
     | [] => []
     | [x] => [x]
   else
     let halves := splitList xs
+    have : xs.length ≥ 2 := by
+      apply Nat.ge_of_not_lt
+      assumption
+    have : halves.fst.length < xs.length := by
+      apply splitList_shorter_fst
+      assumption
+    have : halves.snd.length < xs.length := by
+      apply splitList_shorter_snd
+      assumption
     merge (mergeSort halves.fst) (mergeSort halves.snd)
+termination_by mergeSort xs => xs.length
+
 
 def sorted (xs : List Nat) : Prop :=
   match xs with
@@ -31,7 +70,11 @@ def sorted (xs : List Nat) : Prop :=
   | _ :: [] => True
   | x :: y :: xs => x <= y /\ sorted (y :: xs)
 
-theorem mergeSort_sorts (xs : List Nat) :
-  sorted (mergeSort xs) := by
-  sorry
 
+#eval mergeSort ["yeaseen", "arafat", "mr", "md"]
+#eval mergeSort [44/11, -4, -0, 2*4]
+
+
+--theorem mergeSort_sorts (xs : List Nat) :
+ -- sorted (mergeSort xs) := by
+--  sorry
